### Electrodynamics preliminaries

Let's consider the Laplace equation:

$$ \nabla^2 \phi = 0 $$

A general solution of the equation in spherical coordinates is given by (cfr. Jackson):

$$ \phi(r,\vartheta, \varphi) = \sum_{l=0}^{+\infty} \sum_{m=-l}^{+l}[A_{lm}r^l + B_{lm}r^{-(l+1)}]Y_{lm}(\vartheta, \varphi) $$

Where $Y_{lm}(\vartheta, \varphi)$ are the spherical harmonics. In the case in which we have cilindrical simmetry $(m=0)$ the solution greatly simplifies :

$$ \phi(r,\vartheta) = \sum_{l=0}^{+\infty}[A_{l}r^l + B_{l}r^{-(l+1)}]P_{l}(\cos\vartheta) $$

Where $P_{l}(\cos\vartheta)$ are the Legendre polynomials. One can find the $A_{l}$ and $B_{l}$ coefficents by imposing the necessary boundary conditions.
We remind that in order to guarantee that the Laplace equation gives an unique solution it must be equipped or with Von Neumann type boundary condition (e.g. specification of the orthogonal electric field on the surface of the volume in which the problem is solved), or with Dirichlet type boundary condition (e.g. specification of the potential on the surface of the volume in which the problem is solved).

### L-SPR (Localized Surface Plasmon Resonance)

#### Quasi-static regime $(R<<\lambda)$ - dipolar approximation

Let's consider an electric plane wave of wavelength $\lambda$ interacting with a spherical nanocluster of radius $R$.
In the quasi-static regime $(R<<\lambda)$ we expect a regular displacement of the electronic cloud, so that this produces an electric oscillating dipole $\bar{p}$.

![[Pasted image 20230325120055.png|400]]

We will have then 2 electric fields, one external that generated the oscillating dipole, and one ''internal'' to the nanocluster, generated by the oscillating dipole. This leads naturally to 2 potentials whic summed must satisfy the Laplace equation with the adequate boundary conditions.
We consider the situation in the picture, where $E_0(t)= E_0e^{i\omega t}$.

![[Pasted image 20230325113727.png|500]]

We have then the following:

$$
\nabla^2\phi = 0 \qquad \mbox{+ Dirichlet boundary condition} $$
 
Where we consider :

$$\phi(r, \vartheta) : \begin{cases}\phi_{in}\ \mbox{if}\ r<R\\\phi_{out}\ \mbox{if}\ r>R \end{cases}$$


Our problem has a cilindrical simmetry, so a general solution for either one of the equation is of the form:

$$  \phi(r,\vartheta) = \sum_{l=0}^{+\infty}[A_{l}r^l + B_{l}r^{-(l+1)}]P_{l}(\cos\vartheta)  $$
So that in general our solution is of the form:

$$\phi(r, \vartheta) : \begin{cases}\phi_{in} = \sum_{l=0}^{+\infty}[A_{l}r^l + K_{l}r^{-(l+1)}]P_{l}(\cos\vartheta) \quad \mbox{if}\ r<R\\\phi_{out}= \sum_{l=0}^{+\infty}[B_{l}r^l + C_{l}r^{-(l+1)}]P_{l}(\cos\vartheta)\quad \mbox{if}\ r>R \end{cases}$$

We begin by a simple consideration on $\phi_{in}$ that will make our calculation easier.
Given the fact that the charge is randomly distributed, there is no net charge on the origin of the sphere. This implies that:

$$ \lim_{r\to 0^+}\phi_{in} = \mbox{constant} \qquad \iff \qquad K_l=0, \  \forall l $$

Otherwise the potential would be divergent.
We now consider the application of the Dirichlet condition.
Considering that $\bar{E} = -\nabla \phi$, we have a constant potential all over the space, namely $\phi_{out} = -E_0(t)z$.
So, a fortiori:

$$ \lim_{r \to \infty} \phi(r,\vartheta) =    -E_0(t)z = -E_0(t)r\cos\vartheta$$

Now we consider the same condition on the formal solution:

$$  \lim_{r \to \infty} \phi(r,\vartheta) = \lim_{r \to \infty} \phi_{out}(r,\vartheta) =  \lim_{r \to \infty}\sum_{l=0}^{+\infty}[B_{l}r^l + C_{l}r^{-(l+1)}]P_{l}(\cos\vartheta) \sim \sum_{l=0}^{+\infty}B_{l}r^l P_{l}(\cos\vartheta) $$

So that by comparison:

$$ B_1 = -E_0(t), \ B_2=0, \dots,B_l=0\qquad \forall l \neq 1 $$

Now we impose continuity condition of the electric fields $\bar{E}$ and $\bar{D}$ on the surface of the nanocluster.
We have for the field $\bar{E}$ that the tangential component must be continuous:

$$ E^{\parallel}_{out} = E^{\parallel}_{in} \qquad \Rightarrow \qquad \lim_{r \to R^-} \left( -\frac{1}{r} \frac{\partial \phi_{in}}{\partial \vartheta} \right) = \lim_{r \to R^+} \left( -\frac{1}{r} \frac{\partial \phi_{out}}{\partial \vartheta} \right)$$

And for the field $\bar{D}$ that the perpendicular component must be continuous:

$$ D^{\perp}_{in} = D^{\perp}_{out} \qquad \Rightarrow \qquad \lim_{r \to R^-} \left( -\varepsilon_0\varepsilon(\omega) \frac{\partial \phi_{in}}{\partial r}\right) = \lim_{r \to R^+} \left( -\varepsilon_0\varepsilon_m \frac{\partial \phi_{out}}{\partial r}\right) $$

==Note that we are using $\varepsilon_r  \equiv \varepsilon(\omega)$ ==
In order to perform this calculations we begin by computing the derivates:

$$ \frac{\partial \phi_{in}}{\partial r} =  \sum_{l=0}^{+\infty}lA_{l}r^{l-1} P_{l}(\cos\vartheta) $$

$$\frac{\partial \phi_{in}}{\partial \vartheta} = \sum_{l=0}^{+\infty}A_{l}r^{l} \frac{\partial P_{l}(\cos\vartheta)}{\partial \vartheta}$$

$$ \frac{\partial \phi_{out}}{\partial r} = \sum_{l=0}^{+\infty}[lB_{l}r^{l-1} -(l+1) C_{l}r^{-(l+2)}]P_{l}(\cos\vartheta)$$

$$ \frac{\partial \phi_{out}}{\partial \vartheta} = \sum_{l=0}^{+\infty}[B_{l}r^l + C_{l}r^{-(l+1)}]\frac{\partial P_{l}(\cos\vartheta)}{\partial \vartheta}$$

If one wish is possible to evaluate the Legendre polynomials derivatives using Rodrigues rapresentation.
Using in the derivation the position $x =  \cos\vartheta$

$$\frac{\partial P_{l}(\cos\vartheta)}{\partial \vartheta} = \frac{\partial P_{l}(\cos\vartheta)}{\partial \cos\vartheta}\frac{\partial \cos\vartheta}{\partial \vartheta} = -\sin \vartheta \frac{\partial}{\partial x}\left( \frac{1}{2^l l!} \frac{d^l}{dx^l} [(x^2-1)^l] \right) = -\sin \vartheta \frac{1}{2^l l!} \frac{d^{l+1} }{dx^{l+1}} [(x^2-1)^l] $$

We know impose the continuity conditions:

- Continuity of the tangential component of the electric field $E^{\parallel}_{out} = E^{\parallel}_{in}$:

$$ \sum_{l=0}^{+\infty}A_{l}R^{l-1} \frac{\partial P_{l}(\cos\vartheta)}{\partial \vartheta} = \sum_{l=0}^{+\infty}[B_{l}R^{l-1} + C_{l}R^{-(l+2)}]\frac{\partial P_{l}(\cos\vartheta)}{\partial \vartheta}$$

$$\sum_{l=0}^{+\infty}A_{l}R^{l-1} = \sum_{l=0}^{+\infty}B_{l}R^{l-1} + C_{l}R^{-(l+2)} $$

- Continuity of the perpendicular component of the dielectric field $D^{\perp}_{in} = D^{\perp}_{out}$: 

$$ \varepsilon_0\varepsilon(\omega)\sum_{l=0}^{+\infty}lA_{l}R^{l-1} P_{l}(\cos\vartheta)= \varepsilon_0\varepsilon_m\sum_{l=0}^{+\infty}[lB_{l}R^{l-1} -(l+1) C_{l}R^{-(l+2)}]P_{l}(\cos\vartheta)$$

$$ \varepsilon_0\varepsilon(\omega)\sum_{l=0}^{+\infty}lA_{l}R^{l-1} = \varepsilon_0\varepsilon_m\sum_{l=0}^{+\infty}lB_{l}R^{l-1} -(l+1) C_{l}R^{-(l+2)}$$

These continuity condition must be valid at the same time:

$$ 
\begin{cases}
\sum_{l=0}^{+\infty}A_{l}R^{l-1} = \sum_{l=0}^{+\infty}B_{l}R^{l-1} + C_{l}R^{-(l+2)}\\
\varepsilon_0\varepsilon(\omega)\sum_{l=0}^{+\infty}lA_{l}R^{l-1} = \varepsilon_0\varepsilon_m\sum_{l=0}^{+\infty}[lB_{l}R^{l-1} -(l+1) C_{l}R^{-(l+2)}]
\end{cases}
$$

For the polynomial identity principle:

$$ 
\begin{cases}
A_{l}R^{l-1} = B_{l}R^{l-1} + C_{l}R^{-(l+2)}\\
\varepsilon(\omega)lA_{l}R^{l-1} = \varepsilon_m[lB_{l}R^{l-1} -(l+1) C_{l}R^{-(l+2)}]
\end{cases}
$$

Due to the condition derived from the Dirichlet condition, we consider the system when:

- $l=1$
Considering $B_1 = -E_0(t)$:

$$ 
\begin{cases}
A_{1} = -E_0+ C_{1}R^{-3}\\
\varepsilon(\omega)A_{1} = \varepsilon_m[-E_0(t) -2 C_{1}R^{-3}]
\end{cases}$$

$$\begin{cases}
A_{1} = \frac{-3\varepsilon_m E_0(t)}{\varepsilon(\omega) + 2 \varepsilon_m} \\
C_{1} = \frac{(\varepsilon(\omega)-\varepsilon_m)R^3E_0(t)}{\varepsilon(\omega) + 2 \varepsilon_m}
\end{cases}$$

- $l \neq 1$
In this case $B_l =0$:

$$ 
\begin{cases}
A_{l}R^{l-1} =  C_{l}R^{-(l+2)}\\
\varepsilon(\omega)lA_{l}R^{l-1} = -\varepsilon_m(l+1) C_{l}R^{-(l+2)}
\end{cases}
$$

From which we imply $A_l=C_l = 0$ for $l \neq 1$.

Finally we can write the final expression for the potentials:

$$\phi(r, \vartheta) : \begin{cases}\phi_{in} = \frac{-3\varepsilon_m E_0(t)}{\varepsilon(\omega) + 2 \varepsilon_m}rP_{1}(\cos\vartheta) \quad \mbox{if}\ r<R\\\phi_{out}= \left[ -E_0(t)r + \frac{(\varepsilon(\omega)-\varepsilon_m)R^3E_0(t)}{\varepsilon(\omega) + 2 \varepsilon_m}r^{-2} \right]P_{1}(\cos\vartheta)\quad \mbox{if}\ r>R \end{cases}$$

$$\phi(r, \vartheta) : \begin{cases}\phi_{in} = \frac{-3\varepsilon_m E_0(t)}{\varepsilon(\omega) + 2 \varepsilon_m}r\cos\vartheta \quad \mbox{if}\ r<R\\\phi_{out}= \left[ -E_0(t)r + \frac{(\varepsilon(\omega)-\varepsilon_m)R^3E_0(t)}{\varepsilon(\omega) + 2 \varepsilon_m}r^{-2} \right]\cos\vartheta\quad \mbox{if}\ r>R \end{cases}$$

$$\phi(r, \vartheta) : \begin{cases}\phi_{in} = \frac{-3\varepsilon_m E_0(t)}{\varepsilon(\omega) + 2 \varepsilon_m}r\cos\vartheta \quad \mbox{if}\ r<R\\\phi_{out}= -E_0(t)r\cos\vartheta + \frac{(\varepsilon(\omega)-\varepsilon_m)R^3E_0(t)}{\varepsilon(\omega) + 2 \varepsilon_m}\frac{r\cos\vartheta}{r^3}\quad \mbox{if}\ r>R \end{cases}$$

This expression is easily convertible in cartesian coordinates:

$$\phi(x,y,z) : \begin{cases}\phi_{in} = \frac{-3\varepsilon_m E_0(t)}{\varepsilon(\omega) + 2 \varepsilon_m}z \quad \mbox{if}\ \sqrt{x^2+y^2+z^2}<R\\\phi_{out}= -E_0(t)z + \frac{(\varepsilon(\omega)-\varepsilon_m)R^3E_0(t)}{\varepsilon(\omega) + 2 \varepsilon_m}\frac{z}{(x^2+y^2+z^2)^{3/2}}\quad \mbox{if}\ \sqrt{x^2+y^2+z^2}>R \end{cases}$$

We can now express this using the fact that a dipole is generated. If one recalls that at great distances from the dipole, i.e. $r >> d$, one can express the dipolar potential as:

$$ \phi_{dip} = \frac{1}{4 \pi \varepsilon_0\varepsilon_m} \frac{\bar{p}\cdot\bar{r}}{r^3} $$

We have that the second term in the RHS in $\phi_{out}$ can be identified as $\phi_{dip}$, so that from the equality :

$$ \frac{1}{4 \pi \varepsilon_0\varepsilon_m} \frac{\bar{p}\cdot\bar{r}}{r^3}=\phi_{dip} = \frac{(\varepsilon(\omega)-\varepsilon_m)R^3E_0(t)}{\varepsilon(\omega) + 2 \varepsilon_m}\frac{r\cos\vartheta}{r^3}$$

One can derive the expression for the dipole momentum:

$$\bar{p} = {4 \pi R^3\varepsilon_0\varepsilon_m} \frac{\varepsilon(\omega)-\varepsilon_m}{\varepsilon(\omega) + 2 \varepsilon_m} \bar{E}_0(t)$$

And moreover find the polarizability $\alpha$ using the expression:

$$ \bar{p} = \alpha \varepsilon_0\varepsilon_m \bar{E}_0(t) \qquad \Rightarrow \qquad\alpha = {4 \pi R^3} \frac{\varepsilon(\omega)-\varepsilon_m}{\varepsilon(\omega) + 2 \varepsilon_m} $$

Upon this considerations, we can finally evaluate the total electric field by using $\bar{E} = -\nabla \phi$
We recall first the nabla expression for spherical coordinates:

$$ \nabla = \left( {\partial  \over \partial r},  {1 \over r}{\partial  \over \partial \vartheta}, \frac{1}{r \sin \vartheta}{\partial  \over \partial \varphi}\right) $$

And the proceed to derivate:

$$\bar{E}_{in} = -\nabla \phi_{in} = \frac{3\varepsilon_m E_0(t)}{\varepsilon(\omega) + 2 \varepsilon_m}\cos\vartheta \ \hat{r} - \frac{3\varepsilon_m E_0(t)}{\varepsilon(\omega) + 2 \varepsilon_m}\sin\vartheta \ \hat{\vartheta} = \frac{3\varepsilon_m E_0(t)}{\varepsilon(\omega) + 2 \varepsilon_m} (\cos\vartheta \ \hat{r}-\sin\vartheta \ \hat{\vartheta}) =  $$

$$ = \frac{3\varepsilon_m E_0(t)}{\varepsilon(\omega) + 2 \varepsilon_m} \hat{z} = \frac{3\varepsilon_m }{\varepsilon(\omega) + 2 \varepsilon_m} \bar{E}_0(t) \equiv f_e \bar{E}_0(t) $$

$$\bar{E}_{out} = -\nabla \phi_{out} =E_0(t)(\cos\vartheta \ \hat{r}-\sin\vartheta \ \hat{\vartheta}) + \frac{(\varepsilon(\omega)-\varepsilon_m)R^3E_0(t)}{\varepsilon(\omega) + 2 \varepsilon_m} \left( \frac{2 \cos \vartheta}{r^3}\hat{r} + \frac{\sin \vartheta}{r^3} \hat{\vartheta} \right) =$$

$$ = \bar{E}_0(t) + \frac{1}{4\pi\varepsilon_0\varepsilon_m}p  \left( \frac{2 \cos \vartheta}{r^3}\hat{r} + \frac{\sin \vartheta}{r^3} \hat{\vartheta} \right) = \bar{E}_0(t) + \frac{1}{4\pi\varepsilon_0\varepsilon_m}  \left( \frac{2 (\bar{p} \cdot \hat{r})\hat{r}}{r^3} + \frac{p}{r^3} \sin \vartheta\hat{\vartheta} \right) = $$

$$\bar{E}_0(t) + \frac{1}{4\pi\varepsilon_0\varepsilon_m}  \left( \frac{2 (\bar{p} \cdot \hat{r})\hat{r}}{r^3} + \frac{p}{r^3} (\cos \vartheta \hat{r} - \hat{z}) \right) = \bar{E}_0(t) + \frac{1}{4\pi\varepsilon_0\varepsilon_m}  \left( \frac{3(\bar{p} \cdot \hat{r})\hat{r} -\bar{p}}{r^3}  \right) $$

Putting all together we have :

$$\bar{E}  = 
\begin{cases} \bar{E}_{in} =  \frac{3\varepsilon_m }{\varepsilon(\omega) + 2 \varepsilon_m} \bar{E}_0(t) \equiv f_e \bar{E}_0(t) \quad \mbox{if}\ r<R \\
\bar{E}_{out} =\bar{E}_0(t) + \frac{1}{4\pi\varepsilon_0\varepsilon_m}  \left( \frac{3(\bar{p} \cdot \hat{r})\hat{r} -\bar{p}}{r^3}  \right) \quad \mbox{if}\ r>R
\end{cases}
$$

##### Near-field properties

We label near-field properties the properties implied by the analysis of $\bar{E}_{in}$.
We call the term $f_e$ enhancement term. The resonance condition is achieved when the term $f_e$ is maximum, and this happen when $|\varepsilon(\omega) + 2 \varepsilon_m|$ is minimum. In the case in which $\Im(\varepsilon(\omega))$ is small or slowly varying, this condition simplyfies to :

$$ \Re(\varepsilon(\omega)) + 2\varepsilon_m =0 $$

Which is called Frohlich resonance condition.
What happen is that the field in the nanocluster is greater than the external field, and this enhancement is maximum when the frequency of the external field meets the Frohlich condition.
We call this phenomenon local field enhancement, and the $\omega$ for which the Frohlich condition is met $\omega_{SPR}$ where SPR stands for surface plasmon resonance.
One can find an easy expression for $\omega_{SPR}$ if we consider the expression for dielectric function from [[Zettelkasten/Master's degree/Solid State Physics/Electron dynamics/Drude Theory]] in the high frequency limit $(\omega>>\gamma)$, typically achieved at optical frequencies.
In that specific case $\varepsilon(\omega) = 1- \frac{\omega_P^2}{\omega^2}$ so that the Frohlich condition can be rewrote as:

$$  1- \frac{\omega_P^2}{\omega_{SPR}^2} + 2\varepsilon_m =0 \qquad \iff \qquad \omega_{SPR} = \frac{\omega_P}{\sqrt{1+2\varepsilon_m}} $$

This enhancement effect decrease abruptly when we consider points outside the nanocluster, as shown in the following plot for the total electric field:

![[Pasted image 20230414104242.png|400]]
Moreover we show plot for specific metals showing the resonance. We see that for some metals, e.g. Ag, we have sharp peaks, and for others, e.g. Au, we have a principal peak, but also secondary ones. We will see in the following that for these metals the dipolar approximation is not a good one, and we must resort to a more sophisticated theory.

![[Pasted image 20230414111622.png|300]]![[Pasted image 20230414111655.png|300]]

##### Far-field properties

We label far-field properties the properties implied by the analysis of $\bar{E}_{out}$.
We begin by calling:

$$ \bar{E}_{incident} \equiv \bar{E}_0(t) \qquad \bar{E}_{scattered}\equiv\frac{1}{4\pi\varepsilon_0\varepsilon_m}  \left( \frac{3(\bar{p} \cdot \hat{r})\hat{r} -\bar{p}}{r^3}  \right)$$

That from now on will be called for simplicity $\bar{E}_{i}$, $\bar{E}_{s}$ respectively. 

Given the fact that we are using the phasor rapresentation for the fields, in order to evaluate the power relative quantities we must use the real part of the fields.
We have that, recalling the definition for the time-averaged Poynting vector:

$$\braket{\bar{S}} = \frac{1}{T} \int_0^T (\bar{E} \times \bar{H})dt = \frac{1}{2} \Re(\bar{E} \times \bar{H}^*)$$

So that, if one want to evaluate $\braket{\bar{S}}_{out}$:

$$\braket{\bar{S}}_{out} = \frac{1}{2} \Re(\bar{E}_{out} \times \bar{H}_{out}^*) = \frac{1}{2} \Re[(\bar{E}_i+\bar{E}_s) \times (\bar{H}_i^*+\bar{H}_s^*)] =  $$

$$ =\frac{1}{2} \Re(\bar{E}_i \times \bar{H}_i^*) + \frac{1}{2} \Re(\bar{E}_s \times \bar{H}_s^*) + \frac{1}{2}\Re[ (\bar{E}_i \times \bar{H}_s^*) +(\bar{E}_s \times \bar{H}_i^*)] =  $$ 
$$=\braket{\bar{S}}_{i} + \braket{\bar{S}}_{s} + \braket{\bar{S}}_{extinction}$$

Now is possible to evaluate the net EM power through a surface like the one fixed in the picture:

![[Pasted image 20230424075054.png|300]]
We fix a direction, specifically we are interested in the net EM power entering the surface, so we use the formula:

$$ W = - \oint_{\Sigma} \braket{\bar{S}} \cdot d\bar{\Sigma} $$

In our specific case the total power is:

$$W_{in} = - \oint_{\Sigma} \braket{\bar{S}}_{out} \cdot d\bar{\Sigma} =- \oint_{\Sigma} (\braket{\bar{S}}_{i} + \braket{\bar{S}}_{s} + \braket{\bar{S}}_{ext}) \cdot d\bar{\Sigma} = W_i + W_s + W_{ext} $$

Is now interesting to make a priori consideration on these quantities, without doing explicit calculations.

First the term $W_i$, given the system simmetry, is always 0, for every choice of an integration surface $\Sigma$ with cylindrical simmetry.
From this we can imply $W_i = 0$, that is that the medium in which the nanocluster is set is non absorbing (as we already said, considering that we have a constant electric field and not a diminishing one).
Secondly, we can imply that $W_s >0$, because the scalar product inside the integral is negative (==questo forse è vero, ma si devono fare i calcoli==)
Lastly the ${W}_ext$ is a mixed term, and the fact that is positive or negative depends from the ratio of $E_{incident}$ and $E_{scattered}$. Given the fact that for the conservation of energy one cannot induce a field greater than the one inducing it, it must be that $W_{ext}>0$, or simply put we have a power loss.
So, in total $W_{in} > 0$.

In virtue of our considerations we can write:

$$ W_s + W_{in} = W_{ext} $$

In order to achieve a proper understanding, these quantities must be normalised by the incoming EM incident intensity:

$$ \frac{W_s}{I_{inc}} + \frac{W_{in}}{I_{inc}} = \frac{W_{ext}}{I_{inc}} \qquad \iff \qquad \sigma_s+ \sigma_{in}= \sigma_{ext}$$

This normalisation gives us the relative cross sections.
It usual in application to renomalise these cross section respect to the nanocluster effective area, in order to give an adimensional coefficent call efficency

$$\frac{\sigma_s}{\pi R^2} + \frac{\sigma_{in}}{\pi R^2} = \frac{\sigma_{ext}}{\pi R^2} \qquad \iff \qquad Q_s+ Q_{in}= Q_{ext}$$

Is now of paramount importance to write an analytic expression for $\sigma_{ext}$.

$$ \sigma_s = \frac{k^4}{6 \pi} |\alpha|^2 $$

$$ \sigma_{in} = k\ \Im(\alpha) $$

$$ \sigma_{ext} =\sigma_s+ \sigma_{in} =9 \frac{\omega}{c}\varepsilon_m^{3/2}V \frac{\Im(\varepsilon)}{(\Re(\varepsilon) + 2 \varepsilon_m)^2 + \Im(\varepsilon)^2} $$
