Let's clarify the meaning of :

$$ \sum_{n=-\infty}^{+\infty} a_n $$

By simply stating its definition. First we consider a succession $\{ a_n \}$ which is bilaterally convergent, i.e we split the succession in 2, $\{ a_n \} = \{ a_{-n} \}+\{ a_n \},\ n \in \mathbb{N}$, where each sub-succession must be convergent in the usual sense.
Then we consider, with the same ansatz: 

$$  \sum_{n=-\infty}^{+\infty} a_n  \equiv  \sum_{n=-\infty}^{-1} a_n + \sum_{n=0}^{+\infty} a_n =  \sum_{n=1}^{+\infty} a_{-n} + \sum_{n=0}^{+\infty} a_n  $$

Note also that in any bilateral series, the summation over an index or its opposite is the same for the rule aforementioned.
