## Exercise 1

A ferromagnetic system is described by the following Hamiltonian on a lattice of coordination number $z$ given by

$$
\mathcal{H} = -\frac{1}{2} \sum_{ij} J_{ij} S_i S_j - H \sum_i S_i \tag{1}
$$

where $S \in \{-1, 3\}$.

(a) Define $m = \langle S_i \rangle$, $h = H / \hat{J}(0)$ and $\theta = k_B T / \hat{J}(0)$ where $\hat{J}(0) = \sum_j J_{ij}$.
Find the dimensionless free energy per site $f = F / (N \hat{J}(0))$ as a function of $\theta$, $h$, and $m$.

(b) Write down the self-consistent mean field equation for $m$.

(c) At $\theta = 0$ there is a first-order transition as a function of field $h$ between the $m = +3$ and $m = -1$ states.  
Find the critical field $h_c$ at $\theta = 0$.

(d) Find the critical point $(\theta_c, h_c)$.

### Solution

a) We proceed with the mean field construction. We consider in the mean field approximation $s_is_j \simeq m(s_i+s_j)-m^2$, so that our Hamiltonian becomes:

$$
-\mathscr{H} = m\sum_{i,j} J_{ij}s_i-\frac{1}{2}m^2\sum_{i,j} J_{ij} - H \sum_i  s_i
$$

And using the given prescriptions:

$$ 
\begin{aligned}
-\mathscr{H} 
&= -\frac{1}{2}Nm^2 \hat{J}(0) +(m\hat{J}(0) +H) \sum_i  s_i 
\end{aligned}
$$

Or


$$ 
\begin{aligned}
-\beta\mathscr{H} 
&= -\frac{1}{2}\beta Nm^2 \hat{J}(0) +\beta(m\hat{J}(0) +H) \sum_i  s_i 
\end{aligned}
$$

Up until here nothing changes in the mean field treatment, apart for the prescription given.
Now we evaluate the partition function:

$$ 
\begin{aligned}
\mathcal{Z} &= \text{Tr}\ e^{-\beta\mathscr{H}} = \sum_{\{s\}}\ e^{-\frac{1}{2}\beta Nm^2 \hat{J}(0) +\beta(m\hat{J}(0) +H) \sum_i  s_i } =\\
&= e^{-\frac{1}{2}\beta Nm^2 \hat{J}(0) }\sum_{\{s\}}e^{\beta(m\hat{J}(0) +H) \sum_i  s_i} = e^{-\frac{1}{2}\beta Nm^2 \hat{J} (0)}\prod_{i}\sum_{\{s\}}e^{\beta(m\hat{J}(0) +H) s_i} = \\
&=e^{-\frac{1}{2}\beta Nm^2 \hat{J}(0) }\sum_{\{s\}}e^{\beta(m\hat{J}(0) +H) s_1}\dots e^{\beta(m\hat{J}(0) +H) s_N} = \\
&=e^{-\frac{1}{2}\beta Nm^2 \hat{J}(0) }\sum_{s_1=-1,3}e^{\beta(m\hat{J}(0) +H) s_1}\dots \sum_{s_N=-1,3}e^{\beta(m\hat{J}(0) +H) s_N} = \\
&=e^{-\frac{1}{2}\beta Nm^2 \hat{J}(0) }\left[e^{-\beta(m\hat{J}(0) +H)} +e^{3\beta(m\hat{J}(0) +H)}\right]^N = \\
&=e^{-\frac{1}{2}\beta Nm^2 \hat{J}(0) - N\beta(m\hat{J}(0) +H)}\left[1 +e^{4\beta(m\hat{J}(0) +H)}\right]^N
\end{aligned}
$$

And from this the free energy by definition

$$\beta F = -\ln \mathcal{Z} \iff \beta F = \frac{1}{2}\beta Nm^2 \hat{J}(0) + N\beta(m\hat{J}(0) +H) -N\ln\left[1 +e^{4\beta(m\hat{J}(0) +H)}\right] $$

Or its reduced counterpart:

$$ f = \frac{1}{2}m^2  + m + h - \vartheta\ln\left[1 +e^{4\beta(m\hat{J}(0) +H)}\right] = \frac{1}{2}m^2  + m + h - \vartheta\ln\left[1 +e^{4\frac{m+h}{\vartheta}} \right] $$

b) We simply evaluate the equilibrium condition:

$$ \frac{\partial f}{ \partial m} = 0 \iff m +1 -\vartheta \frac{ \frac{4}{\vartheta}e^{4\frac{m+h}{\vartheta}}}{1 +e^{4\frac{m+h}{\vartheta}}} = 0  \iff m =\frac{ 4e^{4\frac{m+h}{\vartheta}}}{1 +e^{4\frac{m+h}{\vartheta}}}-1  = \frac{ 3e^{4\frac{m+h}{\vartheta}}-1}{1 +e^{4\frac{m+h}{\vartheta}}}  $$

So the self consistent equation is :

$$ m=\frac{ 3e^{4\frac{m+h}{\vartheta}}-1}{1 +e^{4\frac{m+h}{\vartheta}}}  $$

c) On the coexistence line the free energies for both phases are equal. 
So:

$$ f_{p1}(\vartheta = 0, m=-1) = f_{p2}(\vartheta = 0, m=3) \iff h_{p1} =h_{p2} +\frac{1}{2}-1-\frac{9}{2}-3 $$

