Let us consider two identical Ising models on the square lattices $\textbf{A}$ and $\textbf{B}$. They are placed along two parallel planes and are subject to the same magnetic field. Let $J$ be the ferromagnetic interaction between spins belonging to the same lattice, and $J_{AB}$ be an antiferromagnetic interaction between the corresponding spins of the two lattices (bottom/top interactions).

The full Hamiltonian is given by:

$$\mathscr{H} = -J \sum_{\braket{i,j}} \left( \sigma^{A}_{i} \sigma^{A}_{j} - \sigma^{B}_{i} \sigma^{B}_{j} \right) + J_{AB} \sum_{i=1}^{N} \sigma^{A}_{i} \sigma^{B}_{i} - H \sum_{i} \left( \sigma^{A}_{i} + \sigma^{B}_{i} \right)
$$
where $J, J_{AB}, H > 0$, and there are $N$ spins for each lattice (i.e., $2N$ spins in total).

For the simplest case where $J=0$, consider the following:

1) Qualitative Description: Describe qualitatively (without calculations) the expected equilibrium phases (most probable distribution of spins) in the low-temperature limit for:
-  $J_{AB} \gg H$
- $J_{AB} \ll H$

2) Partition Function and Free Energy: Compute exactly the partition function and the limiting free energy of the system.

3) Thermal Averages: Compute exactly the thermal averages $\langle \sigma^A + \sigma^B \rangle$ and $\langle \sigma^A \sigma^B \rangle$. By noticing that $\langle \sigma^A \rangle = \langle \sigma^B \rangle$, obtain $m_A = \langle \sigma^A \rangle$ and $m_B = \langle \sigma^B \rangle$.

4) Low-Temperature Behavior: Study the low-temperature ($\beta \gg 1$) behavior of $m_A = \langle \sigma^A \rangle$ and $\langle \sigma^A \sigma^B \rangle$ in the following three cases:
- $|H| < J_{AB}$
- $H > J_{AB}$
- $H = J_{AB}$

Comments:
- Note that $J=0$, so the first term in $\mathscr{H}$ is zero.
- The spin variables take values $\sigma^A = \pm 1$ and $\sigma^B = \pm 1$.

### Solution

1)  Consider the case $J_{AB} \gg H$. Then the Hamiltonian reduces to $\mathscr{H} \simeq  J_{AB} \sum_{i=1}^{N} \sigma^{A}_{i} \sigma^{B}_{i}$. 
Then the lowest energy configurations are the one with the antiparallel spins, hence this configuration is favored in this regime.
Consider now the case $J_{AB} \ll H$. Then the Hamiltonian reduces to $\mathscr{H} \simeq - H \sum_{i} \left( \sigma^{A}_{i} + \sigma^{B}_{i} \right)$. 
Then the lowest energy configurations are the one with the parallel spins, hence this configuration is favored in this regime.

2) We have:

$$
\begin{aligned}
\mathcal{Z}_N &= \text{Tr}\ e^{-\beta \mathscr{H}} = \sum_{\{\sigma^A\}}\sum_{\{\sigma^B\}}e^{-\beta ( J_{AB} \sum_{i=1}^{N} \sigma^{A}_{i} \sigma^{B}_{i} - H \sum_{i} \left( \sigma^{A}_{i} + \sigma^{B}_{i} \right))} = \prod_{i=1}^N \sum_{\sigma^A_i=\pm1} \sum_{\sigma^B_i=\pm1}e^{-\beta J_{AB}\sigma^{A}_{i} \sigma^{B}_{i} +\beta H  \left( \sigma^{A}_{i} + \sigma^{B}_{i} \right)} =\\
&= \prod_{i=1}^N \sum_{\sigma^A_i=\pm1} e^{-\beta J_{AB}\sigma^{A}_{i} +\beta H  \left( \sigma^{A}_{i} + 1 \right)} + e^{+\beta J_{AB}\sigma^{A}_{i} +\beta H  \left( \sigma^{A}_{i} - 1 \right)} =\\
&= \prod_{i=1}^N  e^{-\beta J_{AB} +2\beta H } +  e^{+\beta J_{AB} } + e^{+\beta J_{AB} } + e^{-\beta J_{AB} -2\beta H } =\\
&= \prod_{i=1}^N    [2e^{+\beta J_{AB} } + e^{-\beta J_{AB}}(2\cosh(2\beta H))  ]=\\
&=  [2e^{+\beta J_{AB} } + e^{-\beta J_{AB}}(2\cosh(2\beta H))  ]^N = e^{+\beta NJ_{AB} }[2 + e^{-2\beta J_{AB}}(2\cosh(2\beta H))  ]^N 
\end{aligned}
$$

And consequently the free energy:

$$ \beta F = -\ln \mathcal{Z} \iff F = -\frac{N}{\beta} \left[ \beta J_{AB } + \ln\left([2 + e^{-2\beta J_{AB}}(2\cosh(2\beta H))  ]  \right) \right] $$

Or the bulk free energy :

$$  f = -J_{AB } - k_BT\ln\left([2 + e^{-2\beta J_{AB}}(2\cosh(2\beta H))]  \right)  $$

3) We have different ansatz:
**First ansatz** : by definition (long and time consuming)
First we show that $\braket{\sigma^A_i} =\braket{\sigma^B_i}$.
By definition of thermal average:

$$ 
\begin{aligned}
\braket{\sigma^A_i} &= \frac{1}{\mathcal{Z_N}}\text{Tr}\ \sigma_i^Ae^{-\beta \mathscr{H}} = \frac{1}{\mathcal{Z_N}}[\text{Tr}_{\{j\neq i\}}\ e^{-\beta E_{pair}} \cdot \text{Tr}_{\{i\}}\sigma_i^Ae^{-\beta E_{pair}} ]  = \\	&=\frac{1}{\mathcal{Z}^N}\left[\mathcal{Z}_{N-1} \sum_{\sigma_{i}^A=\pm1}\sum_{\sigma^B_{i}=\pm1}\sigma_i^Ae^{-\beta E_{pair}} \right] = \frac{1}{\mathcal{Z}^1}\left[2 e^{-\beta J_{AB}} \sinh(2\beta H)\right] = \\
&= \frac{2 e^{-\beta J_{AB}} \sinh(2\beta H)}{e^{+\beta J_{AB} }[2 + e^{-2\beta J_{AB}}(2\cosh(2\beta H))  ] } = m
\end{aligned}
$$

By simmetry I get $\braket{\sigma^B_i} = m$ as the thermal average is functionally equivalent. and $E_{pair}$ is invariant under lattice swap. Then, clearly:

$$ \braket{\sigma^A_i+\sigma^B_i} = \braket{\sigma^A_i}+ \braket{\sigma^B_i} = 2m  $$

Finally, we can evaluate $\braket{\sigma^A_i\sigma^B_i}$ using the definition and the same reasoning as the one before:

$$ \braket{\sigma^A_i\sigma^B_i} = \frac{1}{\mathcal{Z}_1} \sum_{\sigma_{i}^A=\pm1}\sum_{\sigma^B_{i}=\pm1}\sigma_i^A\sigma_i^Be^{-\beta E_{pair}} = \frac{e^{-2\beta J_{AB}}(2\cosh(2\beta H)) -2 }{2 + e^{-2\beta J_{AB}}(2\cosh(2\beta H))  } $$

**Second ansatz** : Using the partition function as a generator (fast)

We observe that this terms appear in the Hamiltonian and thus in the partition function.
We perform the following derivatives:

$$ 
\begin{aligned}
\frac{\partial\ln Z_N}{\partial H} &= \frac{1}{\mathcal{Z}_N}\frac{\partial\mathcal{Z}}{\partial H} = \frac{1}{\mathcal{Z}_N}\frac{\partial}{\partial H} \sum_{\{\sigma^A\}}\sum_{\{\sigma^B\}}e^{-\beta ( J_{AB} \sum_{i=1}^{N} \sigma^{A}_{i} \sigma^{B}_{i} - H \sum_{i} \left( \sigma^{A}_{i} + \sigma^{B}_{i} \right))} =  \\
&= \frac{1}{\mathcal{Z}_N} \sum_{\{\sigma^A\}}\sum_{\{\sigma^B\}}\beta \sum_{i} \left( \sigma^{A}_{i} + \sigma^{B}_{i}\right) e^{-\beta ( J_{AB} \sum_{i=1}^{N} \sigma^{A}_{i} \sigma^{B}_{i} - H \sum_{i} \left( \sigma^{A}_{i} + \sigma^{B}_{i} \right))} = \\
&=\beta \sum_{i} \braket{\sigma^{A}_{i} + \sigma^{B}_{i}}
\end{aligned}
$$

Assuming translational invariance:

$$ \frac{\partial\ln Z_N}{\partial H}= \beta N \braket{\sigma^{A} + \sigma^{B}}  \iff  -\frac{\partial f}{\partial H}=  \braket{\sigma^{A} + \sigma^{B}}  $$

With the same reasoning is easy to show that:

$$ \frac{\partial\ln Z_N}{\partial J_{AB}}= -\beta N \braket{\sigma^{A} \sigma^{B}}  \iff  \frac{\partial f}{\partial J_{AB}}=  \braket{\sigma^{A} \sigma^{B}}  $$

Then one simply does the derivatives.
As we noticed that $\langle \sigma^A \rangle = \langle \sigma^B \rangle = m$, then $\braket{\sigma^{A} + \sigma^{B}} = 2m$.

4) Consider the expressions we obtained:

$$m =\frac{2\sinh(2\beta H)}{e^{+2\beta J_{AB} }[2 + e^{-2\beta J_{AB}}(2\cosh(2\beta H))  ] } \qquad \braket{\sigma^A\sigma^B} = \frac{e^{-2\beta J_{AB}}(2\cosh(2\beta H)) -2 }{2 + e^{-2\beta J_{AB}}(2\cosh(2\beta H))  } $$

Case 1: $|H| < J_{AB}$ (Coupling dominates)
  In this case, $J_{AB} > H > 0$. Therefore, the term $e^{2\beta J_{AB}}$ will grow faster and be dominant over $e^{2\beta H}$ as $\beta \to \infty$.
  Magnetization $m_A$:
  $$m_A = \frac{\sinh(2\beta H)}{e^{2\beta J_{AB}} + \cosh(2\beta H)} \approx \frac{\frac{1}{2}e^{2\beta H}}{e^{2\beta J_{AB}} + \frac{1}{2}e^{2\beta H}}$$
 
 To evaluate the limit, we divide the numerator and denominator by the largest term, $e^{2\beta J_{AB}}$:
  $$m_A \approx \frac{\frac{1}{2}e^{2\beta (H - J_{AB})}}{1 + \frac{1}{2}e^{2\beta (H - J_{AB})}}$$

Since $H - J_{AB} < 0$, in the limit $\beta \to \infty$, the term $e^{2\beta (H - J_{AB})} \to 0$.
  $$\lim_{\beta \to \infty} m_A = \frac{0}{1 + 0} = 0$$

Correlation $\langle \sigma^A \sigma^B \rangle$:
  $$\langle \sigma^A \sigma^B \rangle = \frac{\cosh(2\beta H) - e^{2\beta J_{AB}}}{\cosh(2\beta H) + e^{2\beta J_{AB}}} \approx \frac{\frac{1}{2}e^{2\beta H} - e^{2\beta
  J_{AB}}}{\frac{1}{2}e^{2\beta H} + e^{2\beta J_{AB}}}$$
  Again, we divide by $e^{2\beta J_{AB}}$:
  $$\langle \sigma^A \sigma^B \rangle \approx \frac{\frac{1}{2}e^{2\beta (H - J_{AB})} - 1}{\frac{1}{2}e^{2\beta (H - J_{AB})} + 1}$$
  
  As $\beta \to \infty$, this becomes:
  $$\lim_{\beta \to \infty} \langle \sigma^A \sigma^B \rangle = \frac{0 - 1}{0 + 1} = -1$$



  Case 2: $H > J_{AB}$ (Field Dominates)
In this case, $H > J_{AB} > 0$. Therefore, the term involving $H$, which is $\cosh(2\beta H) \approx \frac{1}{2}e^{2\beta H}$, is the dominant one.


Magnetization $m_A$:
  $$m_A = \frac{\sinh(2\beta H)}{e^{2\beta J_{AB}} + \cosh(2\beta H)} \approx \frac{\frac{1}{2}e^{2\beta H}}{e^{2\beta J_{AB}} + \frac{1}{2}e^{2\beta H}}$$
  
This time, we divide by the largest term, $e^{2\beta H}$:
  $$m_A \approx \frac{\frac{1}{2}}{e^{2\beta (J_{AB} - H)} + \frac{1}{2}}$$

Since $J_{AB} - H < 0$, in the limit $\beta \to \infty$, the term $e^{2\beta (J_{AB} - H)} \to 0$.
  $$\lim_{\beta \to \infty} m_A = \frac{\frac{1}{2}}{0 + \frac{1}{2}} = 1$$

  Correlation $\langle \sigma^A \sigma^B \rangle$:
  $$\langle \sigma^A \sigma^B \rangle = \frac{\cosh(2\beta H) - e^{2\beta J_{AB}}}{\cosh(2\beta H) + e^{2\beta J_{AB}}} \approx \frac{\frac{1}{2}e^{2\beta H} - e^{2\beta
  J_{AB}}}{\frac{1}{2}e^{2\beta H} + e^{2\beta J_{AB}}}$$
  
Divide by $e^{2\beta H}$:

$$\langle \sigma^A \sigma^B \rangle \approx \frac{\frac{1}{2} - e^{2\beta (J_{AB} - H)}}{\frac{1}{2} + e^{2\beta (J_{AB} - H)}}$$

As $\beta \to \infty$, this becomes:

$$\lim_{\beta \to \infty} \langle \sigma^A \sigma^B \rangle = \frac{\frac{1}{2} - 0}{\frac{1}{2} + 0} = 1$$

Case 3: $H = J_{AB}$ (Critical Point)
This is a special case where we set $H = J_{AB}$ before taking the limit.
Magnetization $m_A$:
  $$m_A = \frac{\sinh(2\beta H)}{e^{2\beta H} + \cosh(2\beta H)} \approx \frac{\frac{1}{2}e^{2\beta H}}{e^{2\beta H} + \frac{1}{2}e^{2\beta H}} =
  \frac{\frac{1}{2}e^{2\beta H}}{\frac{3}{2}e^{2\beta H}}$$
  $$\lim_{\beta \to \infty} m_A = \frac{1/2}{3/2} = \frac{1}{3}$$

Correlation $\langle \sigma^A \sigma^B \rangle$:

$$\langle \sigma^A \sigma^B \rangle = \frac{\cosh(2\beta H) - e^{2\beta H}}{\cosh(2\beta H) + e^{2\beta H}} \approx \frac{\frac{1}{2}e^{2\beta H} - e^{2\beta
  H}}{\frac{1}{2}e^{2\beta H} + e^{2\beta H}} = \frac{-\frac{1}{2}e^{2\beta H}}{\frac{3}{2}e^{2\beta H}}$$

$$\lim_{\beta \to \infty} \langle \sigma^A \sigma^B \rangle = \frac{-1/2}{3/2} = -\frac{1}{3}$$

